VNM.v.d
@@ -1,0 +1,2 @@
+VNM.vo VNM.glob VNM.v.beautified: VNM.v ./ATL.vo
+VNM.vio: VNM.v ./ATL.vio
