ATL.v
@@ -5,6 +5,8 @@ Parameter State : Set.
 Parameter Player : Set.
 Parameter Observable : Set.
 
+Parameter beq_player : Player -> Player -> bool.
+
 
 Definition move_number : Set := State -> Player -> nat.
 
@@ -156,11 +158,30 @@ Definition computation_prefix
 
 Check computation_prefix.
 
-Definition strategy (g:CGS) (p:Player) : Type := forall (q:State) (l:computation g q), (@move g.(m) (last (proj1_sig l) q) p).
+Definition strategy (g:CGS) (p:Player) : Set := forall (q:State) (l:computation g q), (@move g.(m) (last (proj1_sig l) q) p).
 
-Definition coalition : Type := Player -> Prop.
+Definition strat_zero (g:CGS) (p:Player) : strategy g p := fun (q:State) => fun (l:computation g q) => 0.
 
-Definition strategy_set (g:CGS) (c:coalition) : Type := forall (p:Player), c p -> @strategy g p.
+Definition coalition : Type := list Player.
+
+Definition grand (g:CGS) : coalition := g.(lp).
+Definition nobody : coalition := nil.
+Definition coal_comp (g:CGS) (c:coalition) : coalition :=
+  let x := fix fx (y z:coalition)
+             := match y with
+                | nil => z
+                | a::y' => if existsb (beq_player a) c then fx y' z else fx y' (a::z)
+                end
+  in x g.(lp) nil.
+
+Definition coal_union (c1 c2 : coalition) : coalition := c1 ++ c2.
+Definition coal_intersection (c1 c2: coalition) : coalition :=
+  let x := fix fx (y1 y2 z: coalition)
+
+
+Definition strategy_set (g:CGS) (c:coalition) : Set := forall (p:Player), c p -> @strategy g p.
+
+Definition ss_zero (g:CGS) (c:coalition) : strategy_set g c := fun (p:Player) => fun (H: (c p)) => strat_zero g p.
 
 Definition outcomes (g:CGS) (q:State) (c:coalition) (ss:strategy_set g c) (l: computation g q)
 :=
@@ -191,9 +212,9 @@ Notation "<< c >>^ p" := (possible_once c  p) (at level 50).
 Notation "<< c >># p" := (possible_always c p) (at level 50).
 Notation "<< c >> p %% q" := (possible_until c p q) (at level 50).
 Notation "[[ c ]]o p" := (possible_next (fun p0:Player => ~(c p0)) p) (at level 50).
-Notation "[[ c ]]^ p" := (possible_once (fun p0:Player => ~(c p0)) p) (at level 50).
-Notation "[[ c ]]# p" := (possible_always (fun p0:Player => ~(c p0)) p) (at level 50).
-Notation "[[ c ]] p %% q" := (possible_until (fun p0:Player => ~(c p0)) p  q) (at level 50).
+Notation "[[ c ]]^ p" := (possible_once (coal_comp c) p) (at level 50).
+Notation "[[ c ]]# p" := (possible_always (coal_comp c) p) (at level 50).
+Notation "[[ c ]] p %% q" := (possible_until (coal_comp c) p  q) (at level 50).
 
 Check forall  (g:CGS) (q:State) (c: coalition),
     exists (ss:strategy_set g c),
@@ -236,10 +257,14 @@ Definition spec : Type := sentence -> Prop.
 
 Definition g_in_spec (sp:spec) (g:CGS) (q:State) : Prop := forall (phi:sentence), sp phi -> verifies g q phi.
 
+
+Axiom dne : forall (phi:sentence), !! (!! phi) = phi.
+Axiom dcomp : forall (c:coalition), coal_comp (coal_comp c) = c.
+
 Theorem coalition_complement_once : forall (g:CGS) (q:State) (phi:sentence) (c:coalition),
-    verifies g q (<<c>>^ phi) <-> verifies g q (lnot ([[c]]^ (lnot phi))).
+    verifies g q (<<c>>^ phi) <-> verifies g q (!! ([[c]]^ (!! phi))).
 Proof.
-  intros g q phi. assert (F: forall (c:coalition), verifies g q (<<c>>^ phi) -> verifies g q (lnot ([[c]]^ (lnot phi)))).
+  intros g q. assert (F: forall (c:coalition) (phi:sentence), verifies g q (<<c>>^ phi) -> verifies g q (!! ([[c]]^ (!! phi)))).
   {
     intros. simpl. simpl in H. unfold not. intros.
     destruct H, H0. assert (P: (computation_property g q (q::nil))).
@@ -248,9 +273,9 @@ Proof.
       - reflexivity.
       - reflexivity.
     }
-    pose ((@exist (list State) (fun l => computation_property g q l) (q::nil) P): computation g q).
-    destruct (H c0). destruct H2. simpl in H2. 
-    destruct (H0 c0). destruct H4. simpl in H4.
+    pose (l:=(@exist (list State) (fun l => computation_property g q l) (q::nil) P): computation g q).
+    destruct (H l). destruct H2. simpl in H2. 
+    destruct (H0 l). destruct H4. simpl in H4.
     destruct x1, x2.
     - apply H4 in H2. apply H2.
     - destruct x2.
@@ -265,5 +290,11 @@ Proof.
       + apply H4 in H2. apply H2.
       + apply H4 in H2. apply H2.
   }
-  assert (B: forall c:coalition, verifies g q (lnot ([[c]]^ (lnot phi))) -> verifies g q (<<c>>^ phi)).
-Admitted.
+  assert (B: forall (c:coalition) (phi:sentence), verifies g q (!! ([[c]]^ (!! phi))) -> verifies g q (<<c>>^ phi)).
+  {
+    intros.
+    pose proof (F (coal_comp c) (!! phi)).
+    rewrite dcomp in H0. rewrite dne in H0.
+    Admitted.
+  }
+  
